Verify correctness of i2c_reg_top
Signed-off-by: Liam Murphy <liampm32@gmail.com>

common/cheshireCircuitScript.sml
@@ -32,11 +32,51 @@ Definition reg_req_decode_def:
 End
 
 Definition reg_rsp_decode_def:
-  reg_rsp_decode (value: 'b word): reg_rsp = <|
+  reg_rsp_decode (value: 34 word): reg_rsp = <|
     rdata := (33 >< 2) value;
     error := word_bit 1 value;
     ready := word_bit 0 value;
   |>
 End
+
+Definition cheshire_req_rel_def:
+  cheshire_req_rel (req_m: (num # num # word32 option) option) (req_c: 'a reg_req) <=>
+  req_c.valid = IS_SOME req_m /\
+  (!nb offset wdata. req_m = SOME (nb, offset, wdata) ==>
+    req_c.write = IS_SOME wdata /\
+    offset = w2n req_c.addr /\
+    (!i. word_bit i req_c.wstrb <=> i < nb) /\
+    (!value. wdata = SOME value ==> req_c.wdata = value))
+End
+
+Theorem cheshire_req_rel_read:
+  cheshire_req_rel (SOME (nb, offset, NONE)) req_c <=>
+  req_c.valid /\ ~req_c.write /\ offset = w2n req_c.addr /\
+  (!i. word_bit i req_c.wstrb <=> i < nb)
+Proof
+  simp [cheshire_req_rel_def]
+QED
+
+Theorem cheshire_req_rel_write:
+  cheshire_req_rel (SOME (nb, offset, SOME wdata)) req_c <=>
+  req_c.valid /\ req_c.write /\ offset = w2n req_c.addr /\ req_c.wdata = wdata /\
+  (!i. word_bit i req_c.wstrb <=> i < nb)
+Proof
+  simp [cheshire_req_rel_def, CONJ_COMM]
+QED
+
+Theorem cheshire_req_rel_valid_write:
+  cheshire_req_rel req_m req_c ==>
+  ((?nb offset wdata. req_m = SOME (nb, offset, SOME wdata)) <=> req_c.valid /\ req_c.write)
+Proof
+  simp [cheshire_req_rel_def]
+  >> rpt strip_tac
+  >> iff_tac
+  >- (rpt strip_tac >> fs [])
+  >- (simp [optionTheory.IS_SOME_EXISTS]
+      >> rpt strip_tac
+      >> PairCases_on `x`
+      >> fs [optionTheory.IS_SOME_EXISTS])
+QED
 
 val _ = export_theory ();
