common/cheshireOracleScript.sml
@@ -1,4 +1,5 @@
 open HolKernel Parse boolLib bossLib;
+open BasicProvers;
 open sharedMemoryOracleTheory;
 
 val _ = new_theory "cheshireOracle";
@@ -64,41 +65,113 @@ Definition cheshire_req_def:
   cheshire_req
     (read_fn: 'ffi -> num -> num -> ffi_outcome + 'notif option # word32)
     (write_fn: 'ffi -> num -> num -> word32 -> ffi_outcome + ('ffi -> 'ffi) # 'notif option)
-    (st: 'ffi) (valid: bool) (write: bool) (nb: num) (offset: num) (wdata: word32) =
-  if ~valid then
-    INR (I, NONE, NONE)
-  else if write then
-    SUM_MAP I (\(st_upd, notif). (st_upd, notif, NONE)) (write_fn st nb offset wdata)
-  else
-    SUM_MAP I (\(notif, rdata). (I, notif, SOME rdata)) (read_fn st nb offset)
+    (st: 'ffi) (req: (num # num # word32 option) option) =
+  case req of
+    NONE => INR (I, NONE, NONE)
+  | SOME (nb, offset, SOME wdata) => SUM_MAP I (\(st_upd, notif). (st_upd, notif, NONE)) (write_fn st nb offset wdata)
+  | SOME (nb, offset, NONE) => SUM_MAP I (\(notif, rdata). (I, notif, SOME rdata)) (read_fn st nb offset)
 End
 
 Theorem cheshire_req_INR_cases:
-  cheshire_req read_fn write_fn st valid write nb offset wdata = INR (st_upd, notif, rdata) ==>
-  (~valid /\ st_upd = I /\ notif = NONE /\ rdata = NONE) \/
-  (valid /\ ~write /\ st_upd = I /\ (?value. rdata = SOME value /\ read_fn st nb offset = INR (notif, value))) \/
-  (valid /\ write /\ rdata = NONE /\ write_fn st nb offset wdata = INR (st_upd, notif))
+  cheshire_req read_fn write_fn st req = INR (st_upd, notif, rdata) ==>
+  (req = NONE /\ st_upd = I /\ notif = NONE /\ rdata = NONE) \/
+  (?nb offset value. req = SOME (nb, offset, NONE) /\ st_upd = I /\ rdata = SOME value /\ read_fn st nb offset = INR (notif, value)) \/
+  (?nb offset wdata. req = SOME (nb, offset, (SOME wdata)) /\ rdata = NONE /\ write_fn st nb offset wdata = INR (st_upd, notif))
 Proof
-  Cases_on `valid`
-  >- (Cases_on `write`
-      >- (Cases_on `write_fn st nb offset wdata`
-          >- simp [cheshire_req_def]
-          >- (Cases_on `y` >> simp [cheshire_req_def]))
-      >- (Cases_on `read_fn st nb offset`
-          >- simp [cheshire_req_def]
-          >- (Cases_on `y` >> simp [cheshire_req_def])))
-  >- simp [cheshire_req_def]
+  simp [cheshire_req_def]
+  >> rpt TOP_CASE_TAC
+  >- (Cases_on `read_fn st q q'`
+      >- simp []
+      >- (Cases_on `y` >> simp []))
+  >- (Cases_on `write_fn st q q' x`
+      >- simp []
+      >- (Cases_on `y` >> simp []))
 QED
 
 Theorem cheshire_req_INR_st_upd_cases:
-  cheshire_req read_fn write_fn st valid write nb offset wdata = INR (st_upd, notif, rdata) ==>
-  (~(valid /\ write) /\ st_upd = I) \/
-  (valid /\ write /\ write_fn st nb offset wdata = INR (st_upd, notif))
+  cheshire_req read_fn write_fn st req = INR (st_upd, notif, rdata) ==>
+  (~(?nb offset wdata. req = SOME (nb, offset, SOME wdata)) /\ st_upd = I) \/
+  (?nb offset wdata. req = SOME (nb, offset, SOME wdata) /\ write_fn st nb offset wdata = INR (st_upd, notif))
 Proof
   rpt strip_tac
-  >> dxrule cheshire_req_INR_cases
-  >> rpt strip_tac
+  >> dxrule_then strip_assume_tac cheshire_req_INR_cases
   >> simp []
+QED
+
+Definition cheshire_run_def:
+  (cheshire_run tick_fn read_fn write_fn st [] = INR (st, [])) /\
+  (cheshire_run tick_fn read_fn write_fn st (req::reqs) =
+    case cheshire_req read_fn write_fn st req of
+      INL x => INL x
+    | INR (st_upd, notif, rdata) => SUM_MAP I (I ## (CONS rdata))
+        (cheshire_run tick_fn read_fn write_fn (st_upd (tick_fn notif st)) reqs))
+End
+
+Theorem ISR_SUM_MAP:
+  !f g z. ISR (SUM_MAP f g z) = ISR z
+Proof
+  Cases_on `z` >> simp []
+QED
+
+Theorem cheshire_run_cheshire_req_ISR:
+  !st reqs.
+  (!st req. MEM req reqs ==> ISR (cheshire_req read_fn write_fn st req)) ==>
+  ISR (cheshire_run tick_fn read_fn write_fn st reqs)
+Proof
+  Induct_on `reqs`
+  >- simp [cheshire_run_def]
+  >- (simp [cheshire_run_def]
+      >> rpt strip_tac
+      >> `?oracle_res. cheshire_req read_fn write_fn st h = INR oracle_res` by simp [GSYM sumExtraTheory.ISR_exists]
+      >> PairCases_on `oracle_res`
+      >> simp [ISR_SUM_MAP])
+QED
+
+Theorem cheshire_run_SNOC:
+  !tick_fn read_fn write_fn st req reqs.
+  cheshire_run tick_fn read_fn write_fn st (SNOC req reqs) =
+  case cheshire_run tick_fn read_fn write_fn st reqs of
+    INL x => INL x
+  | INR (st', rdatas) =>
+    case cheshire_req read_fn write_fn st' req of
+      INL x => INL x
+    | INR (st_upd, notif, rdata) => INR (st_upd (tick_fn notif st'), SNOC rdata rdatas)
+Proof
+  Induct_on `reqs`
+  >- simp [cheshire_run_def]
+  >- (simp [cheshire_run_def]
+      >> rpt strip_tac
+      >> Cases_on `cheshire_req read_fn write_fn st h`
+      >- simp []
+      >- (PairCases_on `y`
+          >> Cases_on `cheshire_run tick_fn read_fn write_fn (y0 (tick_fn y1 st)) reqs`
+          >- simp []
+          >- (PairCases_on `y`
+              >> Cases_on `cheshire_req read_fn write_fn y0' req`
+              >- simp []
+              >- (PairCases_on `y` >> simp []))))
+QED
+
+Theorem cheshire_run_LENGTH_rdatas:
+  !tick_fn read_fn write_fn st reqs st' rdatas.
+  cheshire_run tick_fn read_fn write_fn st reqs = INR (st', rdatas) ==>
+  LENGTH rdatas = LENGTH reqs
+Proof
+  Induct_on `reqs`
+  >- simp [cheshire_run_def]
+  >- (simp [cheshire_run_def]
+      >> rpt strip_tac
+      >> Cases_on `cheshire_req read_fn write_fn st h`
+      >- fs []
+      >- (PairCases_on `y`
+          >> Cases_on `cheshire_run tick_fn read_fn write_fn (y0 (tick_fn y1 st)) reqs`
+          >- fs []
+          >- (PairCases_on `y`
+              >> fs []
+              >> qpat_x_assum `_ = rdatas` (assume_tac o GSYM)
+              >> simp []
+              >> last_x_assum $ drule_then assume_tac
+              >> simp [])))
 QED
 
 val _ = export_theory ();
