i2c/i2cRegsCircuitProofScript.sml
@@ -138,11 +138,11 @@ QED
 val all_ones_rewrites = map (fn n => ``-1w: ^(n |> Arbnum.fromInt |> fcpLib.index_type |> ty_antiq) word`` |> EVAL |> GSYM |> Once) [1, 2, 3, 4];
 
 Theorem i2c_req_error_i2c_write:
-  !(req: 7 reg_req) st nb.
-  req.valid /\ req.write /\ (∀i. word_bit i req.wstrb ⇔ i < nb) ==>
-  i2c_req_error req = ISL (i2c_write st nb (w2n req.addr) req.wdata)
+  cheshire_req_rel (SOME (nb, offset, SOME wdata)) req ==>
+  ISL (i2c_write st nb offset wdata) = i2c_req_error req
 Proof
-  rpt strip_tac
+  simp [cheshire_req_rel_write]
+  >> rpt strip_tac
   >> asm_simp_tac std_ss [i2c_write_def, dimword_def, dimindex_7, w2n_eq_iff_eq_n2w]
   >> rpt TOP_CASE_TAC
   >> simp [i2c_req_error_def]
@@ -154,21 +154,59 @@ Proof
 QED
 
 Theorem i2c_req_error_i2c_read:
-  !(req: 7 reg_req) st nb.
-  req.valid /\ ~req.write ==>
-  i2c_req_error req = ISL (i2c_read st nb (w2n req.addr))
+  cheshire_req_rel (SOME (nb, offset, NONE)) req ==>
+  ISL (i2c_read st nb offset) = i2c_req_error req
 Proof
-  rpt strip_tac
+  simp [cheshire_req_rel_read]
+  >> rpt strip_tac
   >> simp [i2c_read_def, w2n_eq_iff_eq_n2w]
   >> rpt IF_CASES_TAC
   >> simp [i2c_req_error_def]
 QED
 
-Theorem i2c_reg_top_rsp_correct_inner:
+Theorem cheshire_req_i2c_req_error:
+  cheshire_req_rel req_m req_c
+  ==> ISL (cheshire_req i2c_read i2c_write st req_m) = i2c_req_error req_c
+Proof
+  rpt strip_tac
+  >> simp [cheshire_req_def]
+  >> rpt TOP_CASE_TAC
+  >- fs [cheshire_req_rel_def, i2c_req_error_def]
+  >- simp [ISL_SUM_MAP, i2c_req_error_i2c_read]
+  >- simp [ISL_SUM_MAP, i2c_req_error_i2c_write]
+QED
+
+Theorem i2c_reg_top_rsp_ready_error_inner:
   let
     i2c = mk_module (procs (ffs1 ++ [i2c_reg_top_ff] ++ ffs2)) (procs ([i2c_reg_top_comb_1] ++ combs ++ [i2c_reg_top_comb_2])) i2c_circuit_init;
     req = reg_req_decode (fext n).reg_req_i: 7 reg_req;
-    oracle_res = cheshire_req i2c_read i2c_write st req.valid req.write nb (w2n req.addr) req.wdata;
+    rsp = reg_rsp_decode (i2c fext fbits n).reg_rsp_o;
+  in
+  (!proc fext s s'. MEM proc (ffs1 ++ ffs2 ++ combs) ==>
+    let
+      s'' = proc fext s s'
+    in
+      s''.reg2hw = s'.reg2hw /\ s''.regs = s'.regs /\ s''.reg_rsp_o = s'.reg_rsp_o
+      /\ s''.addr = s'.addr /\ s''.write = s'.write /\ s''.wdata = s'.wdata
+      /\ s''.wstrb = s'.wstrb /\ s''.valid = s'.valid)
+  ==> rsp.ready /\ rsp.error = i2c_req_error req
+Proof
+  qpat_abbrev_tac `sstep = procs (_ ++ ffs2)`
+  >> qpat_abbrev_tac `cstep = procs (_ ++ [i2c_reg_top_comb_2])`
+  >> `?s'. mk_circuit sstep cstep (i2c_circuit_init fbits) fext n = cstep (fext n) s' s'` by irule mk_circuit_cstep
+  >> simp [mk_module_def]
+  >> unabbrev_all_tac
+  >> simp [procs_append, procs_def, i2c_reg_top_comb_2_flat]
+  >> simp [procs_unchanged, i2c_reg_top_comb_1_flat, reg_rsp_decode_def, word_bit_bit_field_insert, word_bit_def, FCP_APPLY_UPDATE_THM_2]
+QED
+
+Theorem i2c_reg_top_rsp_ready_error = SRULE [SF boolSimps.LET_ss] i2c_reg_top_rsp_ready_error_inner;
+
+Theorem i2c_reg_top_rsp_correct_inner:
+  let
+    i2c = mk_module (procs (ffs1 ++ [i2c_reg_top_ff] ++ ffs2)) (procs ([i2c_reg_top_comb_1] ++ combs ++ [i2c_reg_top_comb_2])) i2c_circuit_init;
+    req_c = reg_req_decode (fext n).reg_req_i: 7 reg_req;
+    oracle_res = cheshire_req i2c_read i2c_write st req_m;
     rsp = reg_rsp_decode (i2c fext fbits n).reg_rsp_o;
   in
   (!proc fext s s'. MEM proc (ffs1 ++ ffs2 ++ combs) ==>
@@ -179,52 +217,46 @@ Theorem i2c_reg_top_rsp_correct_inner:
       /\ s''.addr = s'.addr /\ s''.write = s'.write /\ s''.wdata = s'.wdata
       /\ s''.wstrb = s'.wstrb /\ s''.valid = s'.valid)
   /\ i2c_state_rel st (i2c fext fbits n)
-  /\ (!i. word_bit i req.wstrb <=> i < nb)
+  /\ cheshire_req_rel req_m req_c
   ==> rsp.ready
     /\ rsp.error = ISL oracle_res
     /\ (!st_upd notif rdata. oracle_res = INR (st_upd, notif, SOME rdata) ==> rsp.rdata = rdata)
 Proof
-  qpat_abbrev_tac `sstep = procs (_ ++ ffs2)`
-  >> qpat_abbrev_tac `cstep = procs (_ ++ [i2c_reg_top_comb_2])`
-  >> simp []
+  simp []
+  >> qpat_abbrev_tac `sstep = procs (_ ++ ffs2)`
+  >> qpat_abbrev_tac `cstep = procs (i2c_reg_top_comb_1::_)`
   >> rpt strip_tac
   >> `?s'. mk_circuit sstep cstep (i2c_circuit_init fbits) fext n = cstep (fext n) s' s'` by irule mk_circuit_cstep
   >> unabbrev_all_tac
-  >> fs [mk_module_def, procs_def, procs_append, reg_rsp_decode_def]
-  (* ready *)
-  >- (simp [i2c_reg_top_comb_2_flat, word_bit_bit_field_insert]
-      >> simp [procs_unchanged, i2c_reg_top_comb_1_flat, word_bit_def, FCP_APPLY_UPDATE_THM_2])
+  >> drule_then assume_tac i2c_reg_top_rsp_ready_error
+  >> simp []
   (* error *)
-  >- (simp [i2c_reg_top_comb_2_flat, word_bit_bit_field_insert]
-      >> simp [procs_unchanged, i2c_reg_top_comb_1_flat, word_bit_def, FCP_APPLY_UPDATE_THM_2, cheshire_req_def]
-      >> rpt IF_CASES_TAC
-      >- simp [i2c_req_error_def]
-      >- fs [ISL_SUM_MAP, i2c_req_error_i2c_write]
-      >- fs [ISL_SUM_MAP, i2c_req_error_i2c_read])
+  >- simp [cheshire_req_i2c_req_error]
   (* rdata *)
-  >- (dep_rewrite.DEP_REWRITE_TAC [i2c_reg_top_comb_2_i2c_read]
-      >> `!fext s s'. (i2c_reg_top_comb_1 fext s s').regs = s'.regs` by simp [i2c_reg_top_comb_1_flat]
-      >> `!fext s s'. (i2c_reg_top_comb_2 fext s s').regs = s'.regs` by simp [i2c_reg_top_comb_2_flat]
-      >> `st.regs = (i2c_reg_top_comb_2 (fext n) s' (procs combs (fext n) s' (i2c_reg_top_comb_1 (fext n) s' s'))).regs` by fs [i2c_state_rel_def, i2c_core_state_rel_def]
-      >> rfs [procs_unchanged]
-      >> `!fext s s'. (i2c_reg_top_comb_2 fext s s').hw2reg = s'.hw2reg` by simp [i2c_reg_top_comb_2_flat]
-      >> `i2c_hwext_read_rel st (i2c_reg_top_comb_2 (fext n) s' (procs combs (fext n) s' (i2c_reg_top_comb_1 (fext n) s' s'))).hw2reg` by fs [i2c_state_rel_def, i2c_core_state_rel_def]
-      >> rfs []
-      >> qabbrev_tac `req = reg_req_decode (fext n).reg_req_i: 7 reg_req`
+  >- (fs [mk_module_def, procs_def, procs_append, reg_rsp_decode_def]
       >> drule_then strip_assume_tac cheshire_req_INR_cases
       >- fs []
-      >- fs [i2c_reg_top_comb_1_flat, optionTheory.SOME_11]
-      >- fs [optionTheory.NOT_SOME_NONE])
+      >- (dep_rewrite.DEP_REWRITE_TAC [i2c_reg_top_comb_2_i2c_read]
+          >> `!fext s s'. (i2c_reg_top_comb_1 fext s s').regs = s'.regs` by simp [i2c_reg_top_comb_1_flat]
+          >> `!fext s s'. (i2c_reg_top_comb_2 fext s s').regs = s'.regs` by simp [i2c_reg_top_comb_2_flat]
+          >> `st.regs = (i2c_reg_top_comb_2 (fext n) s' (procs combs (fext n) s' (i2c_reg_top_comb_1 (fext n) s' s'))).regs` by fs [i2c_state_rel_def, i2c_core_state_rel_def]
+          >> rfs [procs_unchanged]
+          >> `!fext s s'. (i2c_reg_top_comb_2 fext s s').hw2reg = s'.hw2reg` by simp [i2c_reg_top_comb_2_flat]
+          >> `i2c_hwext_read_rel st (i2c_reg_top_comb_2 (fext n) s' (procs combs (fext n) s' (i2c_reg_top_comb_1 (fext n) s' s'))).hw2reg` by fs [i2c_state_rel_def, i2c_core_state_rel_def]
+          >> gs [cheshire_req_rel_read]
+          >> simp [i2c_reg_top_comb_1_flat, cheshire_req_def])
+      >- fs [])
 QED
 
-Theorem i2c_reg_top_rsp_correct = SIMP_RULE (pure_ss ++ boolSimps.LET_ss) [] i2c_reg_top_rsp_correct_inner;
+Theorem i2c_reg_top_rsp_correct = SRULE [SF boolSimps.LET_ss] i2c_reg_top_rsp_correct_inner;
 
 Theorem i2c_write_i2c_hwext_notif_rel:
-  req.valid /\ req.write /\ (∀i. word_bit i req.wstrb ⇔ i < nb) /\
-  i2c_write st nb (w2n req.addr) req.wdata = INR (_, notif) ==>
+  cheshire_req_rel (SOME (nb, offset, SOME wdata)) req /\
+  i2c_write st nb offset wdata = INR (_, notif) ==>
   i2c_hwext_notif_rel notif req
 Proof
-  pure_rewrite_tac [i2c_write_def]
+  simp [cheshire_req_rel_write]
+  >> pure_rewrite_tac [i2c_write_def]
   >> rpt TOP_CASE_TAC
   >> rpt strip_tac
   >> fs [i2c_hwext_notif_rel_def, i2c_req_error_def, w2n_eq_iff_eq_n2w]
@@ -236,11 +268,12 @@ Proof
 QED
 
 Theorem i2c_read_i2c_hwext_notif_rel:
-  req.valid /\ ~req.write /\
-  i2c_read st nb (w2n req.addr) = INR (notif, _) ==>
+  cheshire_req_rel (SOME (nb, offset, NONE)) req /\
+  i2c_read st nb offset = INR (notif, _) ==>
   i2c_hwext_notif_rel notif req
 Proof
-  pure_rewrite_tac [i2c_read_def]
+  simp [cheshire_req_rel_read]
+  >> pure_rewrite_tac [i2c_read_def]
   >> rpt TOP_CASE_TAC
   >> fs [i2c_hwext_notif_rel_def, i2c_req_error_def, w2n_eq_iff_eq_n2w]
 QED
@@ -270,38 +303,13 @@ Proof
   >> simp [procs_unchanged, i2c_reg_top_comb_1_flat]
 QED
 
-Theorem i2c_req_fext = SIMP_RULE (pure_ss ++ boolSimps.LET_ss) [] i2c_req_fext_inner;
-
-Theorem i2c_rsp_i2c_req_error_inner:
-  let
-    i2c = mk_module (procs (ffs1 ++ [i2c_reg_top_ff] ++ ffs2)) (procs ([i2c_reg_top_comb_1] ++ combs ++ [i2c_reg_top_comb_2])) i2c_circuit_init;
-    req = reg_req_decode (fext n).reg_req_i: 7 reg_req;
-  in
-  (!proc fext s s'. MEM proc (ffs1 ++ ffs2 ++ combs) ==>
-    let
-      s'' = proc fext s s'
-    in
-      s''.reg2hw = s'.reg2hw /\ s''.regs = s'.regs /\ s''.reg_rsp_o = s'.reg_rsp_o
-      /\ s''.addr = s'.addr /\ s''.write = s'.write /\ s''.wdata = s'.wdata
-      /\ s''.wstrb = s'.wstrb /\ s''.valid = s'.valid)
-  ==> word_bit 1 (i2c fext fbits n).reg_rsp_o = i2c_req_error req
-Proof
-  qpat_abbrev_tac `sstep = procs (_ ++ ffs2)`
-  >> qpat_abbrev_tac `cstep = procs (_ ++ [i2c_reg_top_comb_2])`
-  >> `?s'. mk_circuit sstep cstep (i2c_circuit_init fbits) fext n = cstep (fext n) s' s'` by irule mk_circuit_cstep
-  >> simp [mk_module_def]
-  >> unabbrev_all_tac
-  >> simp [procs_append, procs_def, i2c_reg_top_comb_2_flat]
-  >> simp [procs_unchanged, i2c_reg_top_comb_1_flat, word_bit_bit_field_insert, word_bit_def, FCP_APPLY_UPDATE_THM_2]
-QED
-
-Theorem i2c_rsp_i2c_req_error = SIMP_RULE (pure_ss ++ boolSimps.LET_ss) [] i2c_rsp_i2c_req_error_inner;
+Theorem i2c_req_fext = SRULE [SF boolSimps.LET_ss] i2c_req_fext_inner;
 
 Theorem i2c_reg_top_i2c_state_rel_step_inner:
-  !ffs1 ffs2 combs fext fbits n st nb st_upd notif rdata.
+  !ffs1 ffs2 combs fext fbits n st req_m st_upd notif rdata.
   let
     i2c = mk_module (procs (ffs1 ++ [i2c_reg_top_ff] ++ ffs2)) (procs ([i2c_reg_top_comb_1] ++ combs ++ [i2c_reg_top_comb_2])) i2c_circuit_init;
-    req = reg_req_decode (fext n).reg_req_i: 7 reg_req;
+    req_c = reg_req_decode (fext n).reg_req_i: 7 reg_req;
   in
   (!proc fext s s'. MEM proc (ffs1 ++ ffs2 ++ combs) ==>
     let
@@ -318,19 +326,20 @@ Theorem i2c_reg_top_i2c_state_rel_step_inner:
    * limitation that you have to know whether something's combinationally or
    * synchronously assigned when using it...) *)
   /\ (!proc fext s s'. MEM proc ffs1 ==> (proc fext s s').hw2reg = s'.hw2reg)
-  /\ (!st fext fbits n st_upd notif rdata.
+  /\ (!st req_m fext fbits n st_upd notif rdata.
     let
-      req = reg_req_decode (fext n).reg_req_i: 7 reg_req
+      req_c = reg_req_decode (fext n).reg_req_i: 7 reg_req
     in
     i2c_state_rel st (i2c fext fbits n)
-    /\ cheshire_req i2c_read i2c_write st req.valid req.write nb (w2n req.addr) req.wdata = INR (st_upd, notif, rdata)
+    /\ cheshire_req_rel req_m req_c
+    /\ cheshire_req i2c_read i2c_write st req_m = INR (st_upd, notif, rdata)
     (* TODO: the other way to do this would be to compare notif to
      * (i2c_reg_top_comb_1 (fext n) (i2c fext fbits n) (i2c fext fbits n)).reg2hw;
      * that has the advantage of being closer to what i2c_core actually operates
      * on, but is also uglier.
      *
      * So, we can try switching to that if this way turns out to be annoying. *)
-    /\ i2c_hwext_notif_rel notif req
+    /\ i2c_hwext_notif_rel notif req_c
     (* Note: somewhat counterintuitively, this actually shows that
      * i2c_hwext_read_rel is true for the next clock cycle, not this one. *)
     ==> ?fnums. i2c_core_state_rel (st_upd (i2c_tick notif (st with fnums := fnums))) (i2c fext fbits (SUC n))
@@ -339,32 +348,30 @@ Theorem i2c_reg_top_i2c_state_rel_step_inner:
       /\ i2c_hw_write_rel (st with fnums := fnums).regs (i2c_tick notif (st with fnums := fnums)).regs
                           (i2c fext fbits n).hw2reg)
   /\ i2c_state_rel st (i2c fext fbits n)
-  /\ (!i. word_bit i req.wstrb <=> i < nb)
-  /\ cheshire_req i2c_read i2c_write st req.valid req.write nb (w2n req.addr) req.wdata = INR (st_upd, notif, rdata)
+  /\ cheshire_req_rel req_m req_c
+  /\ cheshire_req i2c_read i2c_write st req_m = INR (st_upd, notif, rdata)
   ==> ?fnums. i2c_state_rel (st_upd (i2c_tick notif (st with fnums := fnums))) (i2c fext fbits (SUC n))
 Proof
-  asm_simp_tac (pure_ss ++ boolSimps.LET_ss) []
+  simp []
   >> rpt strip_tac
 
-  >> drule_all_then assume_tac i2c_reg_top_rsp_correct
+  >> drule_all_then strip_assume_tac i2c_reg_top_rsp_correct
   >> drule_then assume_tac i2c_req_fext
-  >> drule_then assume_tac i2c_rsp_i2c_req_error
+  >> drule_then assume_tac i2c_reg_top_rsp_ready_error
 
-  >> qabbrev_tac `req = reg_req_decode (fext n).reg_req_i: 7 reg_req`
+  >> qabbrev_tac `req_c = reg_req_decode (fext n).reg_req_i: 7 reg_req`
 
-  >> `i2c_hwext_notif_rel notif req`
-     by (drule cheshire_req_INR_cases
-         >> rpt strip_tac
-         >- simp [i2c_hwext_notif_rel_def, i2c_req_error_def]
-         >- (drule_all i2c_read_i2c_hwext_notif_rel >> simp [])
-         >- (drule_all i2c_write_i2c_hwext_notif_rel >> simp []))
+  >> `i2c_hwext_notif_rel notif req_c`
+     by (drule_then strip_assume_tac cheshire_req_INR_cases
+         >- fs [cheshire_req_rel_def, i2c_hwext_notif_rel_def, i2c_req_error_def]
+         >- (fs [] >> drule_all i2c_read_i2c_hwext_notif_rel >> simp [])
+         >- (fs [] >> drule_all i2c_write_i2c_hwext_notif_rel >> simp []))
 
-  (* We need to do this in all cases so we can pick the value of `fnums`. *)
-  >> fs [Abbr `req`]
-  >> qpat_x_assum `!st fext fbits n st_upd notif rdata. _ ==> ?fnums. _`
-       $ drule_all_then
-       $ qx_choose_then `fnums` assume_tac
-  >> qabbrev_tac `req = reg_req_decode (fext n).reg_req_i: 7 reg_req`
+  (* We need to do this in all cases so we can pick the value of fnums. *)
+  >> fs [Abbr `req_c`]
+  >> qpat_x_assum `!st nb fext fbits n st_upd notif rdata. _ ==> ?fnums. _`
+       $ drule_all_then strip_assume_tac
+  >> qabbrev_tac `req_c = reg_req_decode (fext n).reg_req_i: 7 reg_req`
   >> qexists `fnums`
 
   >> simp [i2c_state_rel_def]
@@ -374,17 +381,17 @@ Proof
   >- (simp [mk_module_def, mk_circuit_def, procs_def, procs_append, i2c_reg_top_comb_2_flat]
       >> simp [procs_unchanged, i2c_reg_top_comb_1_flat]
 
-      >> drule cheshire_req_INR_st_upd_cases
-      >> rpt strip_tac
+      >> drule_then strip_assume_tac cheshire_req_INR_st_upd_cases
 
       >> simp [GSYM mk_module_def]
       >> qpat_abbrev_tac `i2c = mk_module _ _ _`
 
-      >- (simp [i2c_reg_top_ff_flat, procs_unchanged]
+      >- (drule_then (fn thm => full_simp_tac pure_ss [thm]) cheshire_req_rel_valid_write
+          >> simp [i2c_reg_top_ff_flat, procs_unchanged]
           (* TODO: auto-generate this (probably need to make a new *Lib.sml to put it in...) *)
           >> simp [i2c_regs_component_equality, i2c_intr_state_component_equality, i2c_intr_enable_component_equality, i2c_ctrl_component_equality, i2c_fdata_component_equality, i2c_fifo_ctrl_component_equality, i2c_ovrd_component_equality, i2c_timing0_component_equality, i2c_timing1_component_equality, i2c_timing2_component_equality, i2c_timing3_component_equality, i2c_timing4_component_equality, i2c_timeout_ctrl_component_equality, i2c_target_id_component_equality, i2c_txdata_component_equality, i2c_host_timeout_ctrl_component_equality]
           >> gs [i2c_state_rel_def, i2c_tick_hwro_unchanged, i2c_hw_write_rel_def])
-      >- (fs []
+      >- (fs [cheshire_req_rel_write]
           >> drule i2c_write_st_upd_alt
           >> simp [i2c_reg_top_ff_flat, procs_unchanged]
           >> fs [i2c_state_rel_def, i2c_tick_hwro_unchanged, i2c_hw_write_rel_def, reg_rsp_decode_def, w2n_eq_iff_eq_n2w]))
@@ -397,13 +404,244 @@ Proof
 
       >> drule_then strip_assume_tac cheshire_req_INR_st_upd_cases
 
-      >- simp [i2c_tick_buffered_notif_NONE]
-      >- (drule i2c_write_st_upd_alt
+      >- (drule_then (fn thm => full_simp_tac pure_ss [thm]) cheshire_req_rel_valid_write
+          >> simp [i2c_tick_buffered_notif_NONE])
+      >- (fs [cheshire_req_rel_write]
+          >> drule i2c_write_st_upd_alt
           >> simp []
           >> rpt (IF_CASES_TAC >- fs [w2n_eq_iff_eq_n2w])
           >> fs [i2c_tick_buffered_notif_NONE, w2n_eq_iff_eq_n2w]))
 QED
 
-Theorem i2c_reg_top_i2c_state_rel_step = SIMP_RULE (pure_ss ++ boolSimps.LET_ss) [] i2c_reg_top_i2c_state_rel_step_inner;
+Theorem i2c_reg_top_i2c_state_rel_step = SRULE [SF boolSimps.LET_ss] i2c_reg_top_i2c_state_rel_step_inner;
+
+Theorem i2c_read_fnums:
+  !st nb offset fnums. i2c_read (st with fnums := fnums) nb offset = i2c_read st nb offset
+Proof
+  asm_simp_tac std_ss [i2c_read_def]
+  >> asm_simp_tac std_ss [i2c_get_status_fmtfull_def, i2c_get_status_rxfull_def, i2c_get_status_fmtempty_def, i2c_get_status_hostidle_def, i2c_get_status_targetidle_def, i2c_get_status_rxempty_def, i2c_get_status_txfull_def, i2c_get_status_acqfull_def, i2c_get_status_txempty_def, i2c_get_status_acqempty_def, i2c_get_rdata_rdata_def, i2c_get_fifo_status_fmtlvl_def, i2c_get_fifo_status_txlvl_def, i2c_get_fifo_status_rxlvl_def, i2c_get_fifo_status_acqlvl_def, i2c_get_val_scl_rx_def, i2c_get_val_sda_rx_def, i2c_get_acqdata_abyte_def, i2c_get_acqdata_signal_def]
+  >> asm_simp_tac std_ss [i2c_state_accfupds]
+QED
+
+Theorem i2c_write_fnums:
+  !st nb offset fnums wdata. i2c_write (st with fnums := fnums) nb offset wdata = i2c_write st nb offset wdata
+Proof
+  asm_simp_tac std_ss [i2c_write_def, i2c_state_accfupds]
+QED
+
+Theorem i2c_cheshire_req_fnums:
+  !st valid write nb offset wdata fnums.
+  cheshire_req i2c_read i2c_write (st with fnums := fnums) req =
+  cheshire_req i2c_read i2c_write st req
+Proof
+  simp [cheshire_req_def, i2c_read_fnums, i2c_write_fnums]
+QED
+
+Theorem i2c_st_upd_unused_fnums:
+  !st valid write nb offset wdata st_upd notif rdata st'.
+  cheshire_req i2c_read i2c_write st req = INR (st_upd, notif, rdata) ==>
+  unused_fnums_ignored st_upd st'
+Proof
+  rpt strip_tac
+  >> drule_then strip_assume_tac cheshire_req_INR_cases
+  >> simp [unused_fnums_ignored_def]
+  >> qexists `0`
+  >- simp [SF ETA_ss]
+  >- simp [SF ETA_ss]
+  >- (drule i2c_write_st_upd_alt >> simp [SF ETA_ss])
+QED
+
+Theorem OUTR_SUM_MAP:
+  !f g z. ISR z ==> OUTR (SUM_MAP f g z) = g (OUTR z)
+Proof
+  Cases_on `z` >> simp []
+QED
+
+Theorem cheshire_run_unused_fnums:
+  !reqs st.
+  (!st req. MEM req reqs ==> ISR (cheshire_req i2c_read i2c_write st req)) ==>
+  unused_fnums_ignored (\st. FST (OUTR (cheshire_run i2c_tick i2c_read i2c_write st reqs))) st
+Proof
+  Induct_on `reqs`
+  >- (simp [unused_fnums_ignored_def]
+      >> rpt strip_tac
+      >> qexists `0`
+      >> simp [cheshire_run_def, SF ETA_ss])
+  >- (simp [cheshire_run_def]
+      >> rpt strip_tac
+      >> `?oracle_res. cheshire_req i2c_read i2c_write st h = INR oracle_res` by simp [GSYM sumExtraTheory.ISR_exists]
+      >> `!st'. (?fnums. st' = st with fnums := fnums) ==> cheshire_req i2c_read i2c_write st' h = INR oracle_res`
+         by (rpt strip_tac >> simp [i2c_cheshire_req_fnums])
+      >> PairCases_on `oracle_res`
+      >> simp [Cong unused_fnums_ignored_cong]
+      >> `(λst'. FST (OUTR (SUM_MAP I (I ## CONS oracle_res2)
+            (cheshire_run i2c_tick i2c_read i2c_write (oracle_res0 (i2c_tick oracle_res1 st')) reqs)))) =
+          (λst'. FST (OUTR (SUM_MAP I (I ## CONS oracle_res2)
+            (cheshire_run i2c_tick i2c_read i2c_write st' reqs))))
+          o oracle_res0
+          o i2c_tick oracle_res1` by simp [combinTheory.o_DEF]
+      >> simp []
+      >> rpt (irule unused_fnums_ignored_comp >> rpt strip_tac)
+      >- simp [cheshire_run_cheshire_req_ISR, OUTR_SUM_MAP]
+      >- (drule i2c_st_upd_unused_fnums >> simp [])
+      >- simp [i2c_tick_unused_fnums])
+QED
+
+Theorem i2c_st_upd_fnums_fupd:
+  cheshire_req i2c_read i2c_write st req = INR (st_upd, notif, rdata) ==>
+  st_upd (st' with fnums := fnums) = st_upd st' with fnums := fnums
+Proof
+  rpt strip_tac
+  >> drule_then strip_assume_tac cheshire_req_INR_cases
+  >- simp []
+  >- simp []
+  >- (drule i2c_write_st_upd_alt >> simp [])
+QED
+
+Theorem i2c_st_upd_fnums:
+  cheshire_req i2c_read i2c_write st req = INR (st_upd, notif, rdata) ==>
+  (st_upd st').fnums = st'.fnums
+Proof
+  rpt strip_tac
+  >> dxrule_then (qspecl_then [`st'`, `st'.fnums`] assume_tac) i2c_st_upd_fnums_fupd
+  >> `!st. st with fnums := st.fnums = st` by simp [i2c_state_component_equality]
+  >> fs []
+  >> last_x_assum (fn thm => simp [Once thm])
+QED
+
+Theorem cheshire_run_unused_fnums_2:
+  !reqs st.
+  (!st req. MEM req reqs ==> ISR (cheshire_req i2c_read i2c_write st req)) ==>
+  ?n st' rdatas. !fnums. (!i. i < n ==> fnums i = st.fnums i) ==>
+  cheshire_run i2c_tick i2c_read i2c_write (st with fnums := fnums) reqs = INR (st' with fnums := (\i. fnums (i + n)), rdatas)
+Proof
+  Induct_on `reqs`
+  >- (rpt strip_tac
+      >> qexistsl [`0`, `st`, `[]`]
+      >> simp [cheshire_run_def, SF ETA_ss])
+  >- (simp [cheshire_run_def]
+      >> rpt strip_tac
+      >> `?oracle_res. cheshire_req i2c_read i2c_write st h = INR oracle_res` by simp [GSYM sumExtraTheory.ISR_exists]
+      >> PairCases_on `oracle_res`
+      >> fs [i2c_cheshire_req_fnums]
+
+      >> qspecl_then [`oracle_res1`, `st`] assume_tac i2c_tick_unused_fnums
+      >> fs [unused_fnums_ignored_def]
+      >> qrefine `n + m`
+      >> simp []
+      >> drule_then assume_tac i2c_st_upd_fnums_fupd
+      >> simp []
+      >> last_x_assum $ qspec_then `oracle_res0 (i2c_tick oracle_res1 st)` strip_assume_tac
+      >> qexists `n'`
+      >> drule_then assume_tac unused_fnums_ignored_fnums_val_inner
+      >> drule_then assume_tac i2c_st_upd_fnums
+      >> fs []
+      >> qexistsl [`st'`, `oracle_res2::rdatas`]
+      >> simp [])
+QED
+
+(* If the initial model state lines up with `i2c_circuit_init`, and all the
+ * requests in `fext` are valid, then the two states will stay lined up from
+ * that point onwards. *)
+Theorem i2c_reg_top_correct:
+  let
+    i2c = mk_module (procs (ffs1 ++ [i2c_reg_top_ff] ++ ffs2)) (procs ([i2c_reg_top_comb_1] ++ combs ++ [i2c_reg_top_comb_2])) i2c_circuit_init
+  in
+  (!proc fext s s'. MEM proc (ffs1 ++ ffs2 ++ combs) ==>
+    let
+      s'' = proc fext s s'
+    in
+      s''.reg2hw = s'.reg2hw /\ s''.regs = s'.regs /\ s''.reg_rsp_o = s'.reg_rsp_o
+      /\ s''.addr = s'.addr /\ s''.write = s'.write /\ s''.wdata = s'.wdata
+      /\ s''.wstrb = s'.wstrb /\ s''.valid = s'.valid)
+  /\ (!proc fext s s'. MEM proc ffs1 ==> (proc fext s s').hw2reg = s'.hw2reg)
+  /\ (!st req_m fext fbits n st_upd notif rdata.
+    let
+      req_c = reg_req_decode (fext n).reg_req_i: 7 reg_req
+    in
+    i2c_state_rel st (i2c fext fbits n)
+    /\ cheshire_req_rel req_m req_c
+    /\ cheshire_req i2c_read i2c_write st req_m = INR (st_upd, notif, rdata)
+    /\ i2c_hwext_notif_rel notif req_c
+    ==> ?fnums. i2c_core_state_rel (st_upd (i2c_tick notif (st with fnums := fnums))) (i2c fext fbits (SUC n))
+      /\ i2c_hw_write_rel (st with fnums := fnums).regs (i2c_tick notif (st with fnums := fnums)).regs
+                          (i2c fext fbits n).hw2reg)
+
+  (* We phrase it this way instead of as i2c_circuit_init fbits so that
+   * combinational signals are set instead of being random values from fbits. *)
+  /\ i2c_state_rel st (i2c fext fbits 0)
+  /\ (!i. i < LENGTH reqs ==>
+    let
+      req = reg_req_decode (fext i).reg_req_i: 7 reg_req;
+    in
+      ~i2c_req_error req /\ cheshire_req_rel (EL i reqs) req)
+
+  ==> ?fnums. let
+      (st', rdatas) = OUTR (cheshire_run i2c_tick i2c_read i2c_write (st with fnums := fnums) reqs)
+    in
+    i2c_state_rel st' (i2c fext fbits (LENGTH reqs))
+    /\ (!i. i < LENGTH reqs ==>
+      let
+        rsp = reg_rsp_decode (i2c fext fbits i).reg_rsp_o;
+      in
+        rsp.ready /\ ~rsp.error /\ (!value. EL i rdatas = SOME value ==> rsp.rdata = value))
+Proof
+  simp []
+  >> rpt strip_tac
+  >> Induct_on `reqs` using listTheory.SNOC_INDUCT
+  >- (drule i2c_reg_top_rsp_ready_error >> fs [cheshire_run_def, i2c_state_rel_fnums])
+  >- (rpt strip_tac
+
+      (* Satisfy the assumptions for our inductive hypothesis, which will tell us the
+       * `fnums` used by `cheshire_run` up until this point. *)
+      >> `!f n. (!i. i < SUC n ==> f i) <=> (!i. i < n ==> f i) /\ f n`
+         by (rpt strip_tac
+             >> iff_tac
+             >- simp []
+             >- (rpt strip_tac >> Cases_on `i = n` >> simp []))
+      >> fs [listTheory.EL_SNOC, listTheory.EL_LENGTH_SNOC]
+
+      (* Show that `cheshire_run = INR _`. *)
+      >> `!st req. MEM req reqs ==> ISR (cheshire_req i2c_read i2c_write st req)`
+         by (simp [listTheory.MEM_EL]
+             >> rpt strip_tac
+             >> qpat_x_assum `!i. i < LENGTH reqs ==> _` $ drule_then strip_assume_tac
+             >> drule cheshire_req_i2c_req_error
+             >> simp [Excl "NOT_ISL_ISR", GSYM sumTheory.NOT_ISL_ISR])
+      >> drule_then (qspecl_then [`i2c_tick`, `st with fnums := fnums`] assume_tac) cheshire_run_cheshire_req_ISR
+      >> drule_then strip_assume_tac (iffLR sumExtraTheory.ISR_exists)
+      >> fs []
+      >> pairarg_tac
+      >> fs []
+
+      (* Infer from `~i2c_req_error` that `cheshire_req = INR _`, so that it can be
+       * used by `drule_all i2c_reg_top_i2c_state_rel_step`. *)
+      >> drule_all_then strip_assume_tac i2c_reg_top_rsp_correct
+      >> drule_then assume_tac i2c_reg_top_rsp_ready_error
+      >> gs []
+      >> drule_then (qx_choose_then `oracle_res` assume_tac) (iffLR sumExtraTheory.ISR_exists)
+      >> PairCases_on `oracle_res`
+      >> drule_all_then strip_assume_tac i2c_reg_top_i2c_state_rel_step
+
+      (* Now we have `fnums'`, the `fnums` needed for the last step to keep things
+       * lining up, and we want to use `qexists` with `fnums'` glued onto the end of
+       * `fnums`. But first, we need to find out where that end is. *)
+      >> `!st req. MEM req reqs ==> ISR (cheshire_req i2c_read i2c_write st req)`
+         by (simp [listTheory.MEM_EL]
+             >> rpt strip_tac
+             >> qpat_x_assum `!i. i < LENGTH reqs ==> _` $ drule_then strip_assume_tac
+             >> drule cheshire_req_i2c_req_error
+             >> simp [Excl "NOT_ISL_ISR", GSYM sumTheory.NOT_ISL_ISR])
+      >> drule_then (qspec_then `st with fnums := fnums` strip_assume_tac) cheshire_run_unused_fnums_2
+      >> qexists `\i. if i < n then fnums i else fnums' (i - n)`
+
+      >> first_assum $ qspec_then `\i. if i < n then fnums i else fnums' (i - n)` assume_tac
+      (* Instantiate it a second time to prove that st'' = st'. *)
+      >> first_x_assum $ qspec_then `fnums` assume_tac
+      >> gs [cheshire_run_SNOC, i2c_cheshire_req_fnums]
+      >> drule_then assume_tac cheshire_run_LENGTH_rdatas
+      >> first_x_assum (assume_tac o GSYM)
+      >> fs [i2c_cheshire_req_fnums, SF ETA_ss, listTheory.EL_SNOC, listTheory.EL_LENGTH_SNOC])
+QED
 
 val _ = export_theory ();
